theories/combined/rules.v
@@ -1,0 +1,62 @@
+From iris.proofmode Require Export tactics.
+From iris.prelude Require Import options.
+From melocoton Require Import named_props multirelations.
+From melocoton.language Require Import language weakestpre.
+From melocoton.interop Require Import basics basics_resources prims_proto.
+From melocoton.lang_to_mlang Require Import lang weakestpre.
+From melocoton.interop Require Import state lang weakestpre update_laws wp_utils wp_simulation.
+From melocoton.ml_lang Require Import primitive_laws lang_instantiation.
+From melocoton.c_lang Require Import lang_instantiation mlang_instantiation.
+From melocoton.mlanguage Require Import progenv.
+From melocoton.mlanguage Require Import weakestpre mlanguage adequacy.
+From melocoton.linking Require Import lang weakestpre.
+
+Notation combined_lang := (link_lang wrap_lang C_mlang).
+Notation combined_prog e p := (link_prog wrap_lang C_mlang (wrap_prog e) p).
+
+Class ffiG `{SI: indexT} (Σ : gFunctors) : Set := FFIG {
+  ffiG_invG :> invG Σ;
+  ffiG_CG :> heapG_C Σ;
+  ffiG_MLG :> heapG_ML Σ;
+  ffiG_wrapperG :> wrapperG Σ;
+  ffiG_linkG :> linkG Σ;
+}.
+
+Section combined_rules.
+Context {SI: indexT}.
+Context `{!ffiG Σ}.
+
+Lemma combined_embed_c (p : lang_prog C_lang) (Ψ Ψ' : protocol C_intf.val Σ) :
+  Ψ ||- p :: Ψ' →
+  Ψ |- (link_lift2 wrap_lang _ p) :: Ψ'.
+Proof.
+  intros H%lang_to_mlang_correct. by apply link_lift2_correct.
+Qed.
+
+Lemma combined_correct
+  (* `{indexT} `{!ffiG Σ} *)
+  (e : ML_lang.expr) (p : lang_prog C_lang)
+  (* (Ψ : ∀ `{!ffiG Σ}, protocol ML_lang.val Σ) *)
+  (Ψ : protocol ML_lang.val Σ)
+  (Pret : Z → Prop)
+:
+  Ψ on prim_names ⊑ ⊥ →
+  dom p ## prim_names →
+  {{{ True }}} e at ⟨∅, Ψ⟩ {{{ x, RET (ML_lang.LitV (ML_lang.LitInt x)); ⌜Pret x⌝ }}} →
+  prims_proto Ψ ||- p :: wrap_proto Ψ →
+  ⊥ |- combined_prog e p :: main_proto Pret.
+Proof.
+  intros.
+  eapply prog_triple_mono_r; swap 1 2.
+  1: eapply link_close_correct.
+  { rewrite dom_prims_prog. set_solver. }
+  1: eapply prog_triple_mono; last by apply wrap_correct.
+  1: reflexivity.
+  1: reflexivity.
+  1: eapply prog_triple_mono; last by apply lang_to_mlang_correct.
+  2: reflexivity.
+  1: by rewrite -proto_refines_join_l.
+  by rewrite -proto_refines_join_l -proto_refines_join_r.
+Qed.
+
+End combined_rules.
